Apply.lean: separate calculation from proof and remove `import all Bdd.Basic`

Bdd/Apply.lean
@@ -1,57 +1,58 @@
 module
 
 public import Bdd.Basic
--- TODO : remove
-import all Bdd.Basic
 import Std.Data.HashMap.Lemmas
 
 namespace Apply
 
 open RawBdd
 
-structure State (n) (n') (m) (m') where
+structure State n n' m m' where
   size : Nat
   heap : Vector (RawNode (max n n')) size
   cache : Std.HashMap (Pointer m × Pointer m') RawPointer
 
-def initial : State n n' m m' := ⟨_, (Vector.emptyWithCapacity (m ⊔ m')), Std.HashMap.emptyWithCapacity (m ⊔ m')⟩
+def initial {n n' m m'} : State n n' m m' :=
+  ⟨_, (Vector.emptyWithCapacity (m ⊔ m')), Std.HashMap.emptyWithCapacity (m ⊔ m')⟩
 
-def Invariant (op : Bool → Bool → Bool) (O : OBdd n m) (U : OBdd n' m') (r : State n n' m m') :=
+def Invariant {n m n' m'} (op : Bool → Bool → Bool) (O_heap : Vector (Node n m) m)
+    (U_heap : Vector (Node n' m') m') (r : State n n' m m') :=
   ∃ hh : (∀ i : Fin r.size, RawNode.Bounded i r.heap[i]),
     ∀ (k : (Pointer m × Pointer m')) (p : RawPointer),
       r.cache[k]? = some p →
       (∀ j h, p = .inr j → (r.heap[j]'h).va.1 =
-        (toVar_or O.1.heap k.1 (n ⊔ n')) ⊓ (toVar_or U.1.heap k.2 (n ⊔ n'))) ∧
-      ∃ hk1 : Bdd.Ordered ⟨O.1.heap, k.1⟩,
-        ∃ hk2 : Bdd.Ordered ⟨U.1.heap, k.2⟩,
+        (toVar_or O_heap k.1 (n ⊔ n')) ⊓ (toVar_or U_heap k.2 (n ⊔ n'))) ∧
+      ∃ hk1 : Bdd.Ordered ⟨O_heap, k.1⟩,
+        ∃ hk2 : Bdd.Ordered ⟨U_heap, k.2⟩,
           ∃ hp : p.Bounded r.size,
             ∃ o : Bdd.Ordered ⟨cook_heap r.heap hh, p.cook hp⟩,
               ∀ I,
                 OBdd.evaluate ⟨⟨cook_heap r.heap hh, p.cook hp⟩, o⟩ I =
                 op
-                  (OBdd.evaluate ⟨⟨O.1.heap, k.1⟩, hk1⟩ (Vector.cast (by simp) (I.take n)))
-                  (OBdd.evaluate ⟨⟨U.1.heap, k.2⟩, hk2⟩ (Vector.cast (by simp) (I.take n')))
+                  (OBdd.evaluate ⟨⟨O_heap, k.1⟩, hk1⟩ (Vector.cast (by simp) (I.take n)))
+                  (OBdd.evaluate ⟨⟨U_heap, k.2⟩, hk2⟩ (Vector.cast (by simp) (I.take n')))
 
-lemma inv_initial {op} {O : OBdd n m} {U : OBdd n' m'} : Invariant op O U initial := by
+lemma inv_initial {n m n' m' op} {O : OBdd n m} {U : OBdd n' m'} : Invariant op O.bdd.heap U.bdd.heap initial := by
   constructor
   · intro k p hp
     simp only [initial, Std.HashMap.getElem?_emptyWithCapacity, reduceCtorEq] at hp
   · rintro ⟨_, c⟩
     simp only [initial, Nat.not_lt_zero] at c
 
-def cache_get (O_root : Pointer m) (U_root : Pointer m') (s : (State n n' m m')) : (Option RawPointer) :=
+def cache_get {m m' n n'} (O_root : Pointer m) (U_root : Pointer m') (s : (State n n' m m')) : (Option RawPointer) :=
   s.cache[(⟨O_root, U_root⟩ : (Pointer m × Pointer m'))]?
 
-lemma heap_push_aux (s : (State n n' m m')) (inv : Invariant op O U s)
+lemma heap_push_aux {n n' m m' op} {O : OBdd n m} {U : OBdd n' m'} {N} (s : (State n n' m m'))
+    (inv : Invariant op O.bdd.heap U.bdd.heap s)
     (hNl : ∃ k : Pointer m × Pointer m', s.cache[k]? = some N.lo)
     (hNh : ∃ k : Pointer m × Pointer m', s.cache[k]? = some N.hi)
     (hNv : N.va.1 = (toVar_or O.1.heap O.1.root (n ⊔ n')) ⊓ (toVar_or U.1.heap U.1.root (n ⊔ n')))
     (hxl : ∀ j h (_ : N.lo = .inr j), N.va.1 < (s.heap[j]'h).va.1)
     (hxh : ∀ j h (_ : N.hi = .inr j), N.va.1 < (s.heap[j]'h).va.1)
     (hh : ∀ h0 (h1 : Bdd.Ordered _) (I : Vector Bool (max n n')),
-            OBdd.evaluate ⟨{ heap := cook_heap (s.heap.push N) h0, root := Pointer.node ⟨s.size, by simp⟩ }, h1⟩ I =
-            op (O.evaluate (Vector.cast (by omega) (I.extract 0 n))) (U.evaluate (Vector.cast (by omega) (I.extract 0 n')))) :
-    Invariant op O U
+      OBdd.evaluate ⟨{ heap := cook_heap (s.heap.push N) h0, root := Pointer.node ⟨s.size, by simp⟩ }, h1⟩ I =
+      op (O.evaluate (Vector.cast (by omega) (I.extract 0 n))) (U.evaluate (Vector.cast (by omega) (I.extract 0 n')))) :
+    Invariant op O.bdd.heap U.bdd.heap
       { size := s.size + 1, heap := s.heap.push N, cache := s.cache.insert (O.1.root, U.1.root) (Sum.inr s.size) } := by
   rcases hNl with ⟨kl, hkl⟩
   rcases hNh with ⟨kh, hkh⟩
@@ -141,8 +142,7 @@ lemma heap_push_aux (s : (State n n' m m')) (inv : Invariant op O U s)
         apply push_ordered
         · exact this
         · exact that.2.1
-      ·
-        simp [Nat.succ_eq_add_one, Bdd.var_eq, cook_heap, Bdd.high_eq, RawPointer.cook]
+      · simp [Nat.succ_eq_add_one, Bdd.var_eq, cook_heap, Bdd.high_eq, RawPointer.cook]
         cases heq : N.hi with
         | inl val =>
           rw [← cook_high]
@@ -196,7 +196,13 @@ lemma heap_push_aux (s : (State n n' m m')) (inv : Invariant op O U s)
         · simp only [RawPointer.cook_equiv]
     exact that.2.2.2.2.2 I
 
-def heap_push (N : RawNode (n ⊔ n')) (s : (State n n' m m')) (inv : Invariant op O U s)
+def heap_push {n n' m m'} (O : OBdd n m) (U : OBdd n' m') (N : RawNode (n ⊔ n'))
+    (s : State n n' m m') : State n n' m m' × RawPointer :=
+  ⟨⟨s.size + 1, s.heap.push N, s.cache.insert ⟨O.1.root, U.1.root⟩ (.inr s.size)⟩, .inr s.size⟩
+
+lemma heap_push_correct {n n' m m' op} {O : OBdd n m} {U : OBdd n' m'} (N : RawNode (n ⊔ n'))
+    {s : State n n' m m'} {r} (heq : r = heap_push O U N s)
+    (inv : Invariant op O.bdd.heap U.bdd.heap s)
     (hNl : ∃ k : Pointer m × Pointer m', s.cache[k]? = some N.lo)
     (hNh : ∃ k : Pointer m × Pointer m', s.cache[k]? = some N.hi)
     (hNv : N.va.1 = (toVar_or O.1.heap O.1.root (n ⊔ n')) ⊓ (toVar_or U.1.heap U.1.root (n ⊔ n')))
@@ -206,43 +212,41 @@ def heap_push (N : RawNode (n ⊔ n')) (s : (State n n' m m')) (inv : Invariant 
             OBdd.evaluate ⟨{ heap := cook_heap (s.heap.push N) h0, root := Pointer.node ⟨s.size, by simp⟩ }, h1⟩ I =
             op (O.evaluate (Vector.cast (by omega) (I.extract 0 n))) (U.evaluate (Vector.cast (by omega) (I.extract 0 n'))))
             (hc : s.cache[(⟨O.1.root, U.1.root⟩ : Pointer m × Pointer m')]? = none ) :
-    { r : State n n' m m' × RawPointer //
-      (Invariant op O U r.1) ∧
-      (r.1.cache[(⟨O.1.root, U.1.root⟩ : Pointer m × Pointer m')]? = some r.2) ∧
-      s.size ≤ r.1.size ∧
-      (∀ (k : Pointer m × Pointer m'),
-        (∀ p, s.cache[k]? = some p → r.1.cache[k]? = some p) ∧
-        (r.1.cache[k]? = none → s.cache[k]? = none) ∧
-        (s.cache[k]? = none → (∃ p, r.1.cache[k]? = some p) → Pointer.Reachable O.1.heap O.1.root k.1 ∧ Pointer.Reachable U.1.heap U.1.root k.2))
-    } :=
-  ⟨⟨⟨s.size + 1, s.heap.push N, s.cache.insert ⟨O.1.root, U.1.root⟩ (.inr s.size)⟩, .inr s.size⟩, by
-    constructor
+    (Invariant op O.bdd.heap U.bdd.heap r.1) ∧
+    (r.1.cache[(⟨O.1.root, U.1.root⟩ : Pointer m × Pointer m')]? = some r.2) ∧
+    s.size ≤ r.1.size ∧
+    (∀ (k : Pointer m × Pointer m'),
+      (∀ p, s.cache[k]? = some p → r.1.cache[k]? = some p) ∧
+      (r.1.cache[k]? = none → s.cache[k]? = none) ∧
+      (s.cache[k]? = none → (∃ p, r.1.cache[k]? = some p) →
+      Pointer.Reachable O.1.heap O.1.root k.1 ∧ Pointer.Reachable U.1.heap U.1.root k.2)) := by
+    subst heq
+    split_ands
     · exact heap_push_aux s inv hNl hNh hNv hxl hxh hh
-    · constructor
-      · simp only [Std.HashMap.getElem?_insert_self]
+    · simp only [heap_push, Std.HashMap.getElem?_insert_self]
+    · simp only [heap_push, Nat.le_add_right]
+    · intro k
+      constructor
+      · intro p hkp
+        rw [← hkp]
+        simp only [heap_push, Std.HashMap.getElem?_insert, beq_iff_eq, ite_eq_right_iff]
+        intro contra
+        rw [← contra] at hkp
+        rw [hkp] at hc
+        contradiction
       · constructor
-        · simp only [Nat.le_add_right]
-        · intro k
-          constructor
-          · intro p hkp
-            rw [← hkp]
-            simp only [Std.HashMap.getElem?_insert, beq_iff_eq, ite_eq_right_iff]
-            intro contra
-            rw [← contra] at hkp
-            rw [hkp] at hc
-            contradiction
-          · constructor
-            · simp only [getElem?_eq_none_iff, Std.HashMap.mem_insert, beq_iff_eq, not_or,
-                and_imp, imp_self, implies_true]
-            · rintro hk ⟨q, hq⟩
-              simp only [Std.HashMap.getElem?_insert, beq_iff_eq] at hq
-              split at hq
-              next heqq => subst heqq; constructor <;> exact .refl
-              next heqq => rw [hk] at hq; contradiction
-  ⟩
+        · simp only [heap_push, getElem?_eq_none_iff, Std.HashMap.mem_insert, beq_iff_eq, not_or,
+            and_imp, imp_self, implies_true]
+        · rintro hk ⟨q, hq⟩
+          simp only [heap_push, Std.HashMap.getElem?_insert, beq_iff_eq] at hq
+          split at hq
+          next heqq => subst heqq; constructor <;> exact .refl
+          next heqq => rw [hk] at hq; contradiction
 
-lemma insert_terminal_invariant (s0 : State n n' m m') (inv : Invariant op O U s0) (ho : O.1.root = .terminal b) (hu : U.1.root = .terminal b'):
-    Invariant op O U { size := s0.size, heap := s0.heap, cache := s0.cache.insert (O.1.root, U.1.root) (Sum.inl (op b b')) } := by
+lemma insert_terminal_invariant {n n' m m' op} {O : OBdd n m} {U : OBdd n' m'} {b b'}
+    (s0 : State n n' m m') (inv : Invariant op O.bdd.heap U.bdd.heap s0)
+    (ho : O.1.root = .terminal b) (hu : U.1.root = .terminal b') :
+    Invariant op O.bdd.heap U.bdd.heap { size := s0.size, heap := s0.heap, cache := s0.cache.insert (O.1.root, U.1.root) (Sum.inl (op b b')) } := by
   constructor
   intro k p hp
   simp only at hp
@@ -287,55 +291,50 @@ lemma op_if3 (op : Bool → Bool → Bool) {c lt lf rt rf : Bool} :
     simp_all only
   next h => simp_all only [Bool.not_eq_true]
 
-lemma aux_lt1_low {O : OBdd n m} {U : OBdd n' m'} (O_root_def : O.1.root = .terminal b) (U_root_def : U.1.root = .node j') :
+lemma aux_lt1_low {n m n' m' b j'} {O : OBdd n m} {U : OBdd n' m'}
+    (O_root_def : O.1.root = .terminal b) (U_root_def : U.1.root = .node j') :
     U.1.heap[j'].var.1 <
     min (toVar_or O.1.heap O.1.root (max n n'))
-        (toVar_or U.1.heap (U.low U_root_def).1.root (max n n')) := by
+        (toVar_or U.1.heap U.bdd.heap[j'].low (max n n')) := by
   have := OBdd.var_lt_low_var (h := U_root_def)
   simp_all [OBdd.var_eq, toVar_or]
   split <;> simp_all
 
-lemma aux_lt1_high {O : OBdd n m} {U : OBdd n' m'} (O_root_def : O.1.root = .terminal b) (U_root_def : U.1.root = .node j') :
+lemma aux_lt1_high {n m n' m' b j'} {O : OBdd n m} {U : OBdd n' m'}
+    (O_root_def : O.1.root = .terminal b) (U_root_def : U.1.root = .node j') :
     U.1.heap[j'].var.1 <
     min (toVar_or O.1.heap O.1.root (max n n'))
-        (toVar_or U.1.heap (U.high U_root_def).1.root (max n n')) := by
+        (toVar_or U.1.heap U.bdd.heap[j'].high (max n n')) := by
   have := OBdd.var_lt_low_var (h := U_root_def)
   have := OBdd.var_lt_high_var (h := U_root_def)
   simp_all [OBdd.var_eq, toVar_or]
   split <;> simp_all
 
-lemma aux_lt2_low {O : OBdd n m} {U : OBdd n' m'} (O_root_def : O.1.root = .node j) (U_root_def : U.1.root = .terminal b') :
+lemma aux_lt2_low {n m n' m' j b'} {O : OBdd n m} {U : OBdd n' m'}
+    (O_root_def : O.1.root = .node j) (U_root_def : U.1.root = .terminal b') :
     O.1.heap[j].var.1 <
-    min (toVar_or O.1.heap (O.low O_root_def).1.root (max n n'))
+    min (toVar_or O.1.heap O.bdd.heap[j].low (max n n'))
         (toVar_or U.1.heap U.1.root (max n n')) := by
   have := OBdd.var_lt_low_var (h := O_root_def)
   have := OBdd.var_lt_high_var (h := O_root_def)
   simp_all [OBdd.var_eq, toVar_or]
   split <;> simp_all
 
-lemma aux_lt2_high {O : OBdd n m} {U : OBdd n' m'} (O_root_def : O.1.root = .node j) (U_root_def : U.1.root = .terminal b') :
+lemma aux_lt2_high {n m n' m' j b'} {O : OBdd n m} {U : OBdd n' m'}
+    (O_root_def : O.1.root = .node j) (U_root_def : U.1.root = .terminal b') :
     O.1.heap[j].var.1 <
-    min (toVar_or O.1.heap (O.high O_root_def).1.root (max n n'))
+    min (toVar_or O.1.heap O.bdd.heap[j].high (max n n'))
         (toVar_or U.1.heap U.1.root (max n n')) := by
   have := OBdd.var_lt_low_var (h := O_root_def)
   have := OBdd.var_lt_high_var (h := O_root_def)
   simp_all [OBdd.var_eq, toVar_or]
   split <;> simp_all
 
-lemma aux_lt3_low {O : OBdd n m} {U : OBdd n' m'} (O_root_def : O.1.root = .node j) (U_root_def : U.1.root = .node j') (hleq : O.1.heap[j].var.1 < U.1.heap[j'].var.1) :
+lemma aux_lt3_low {n m n' m' j j'} {O : OBdd n m} {U : OBdd n' m'}
+    (O_root_def : O.1.root = .node j) (U_root_def : U.1.root = .node j')
+    (hleq : O.1.heap[j].var.1 < U.1.heap[j'].var.1) :
     O.1.heap[j].var.1 <
-    min (toVar_or O.1.heap (O.low O_root_def).1.root (max n n'))
-        (toVar_or U.1.heap U.1.root (max n n')) := by
-  have := OBdd.var_lt_low_var (h := O_root_def)
-  have := OBdd.var_lt_high_var (h := O_root_def)
-  have := OBdd.var_lt_low_var (h := U_root_def)
-  have := OBdd.var_lt_high_var (h := U_root_def)
-  simp_all [OBdd.var_eq, toVar_or]
-  split <;> simp_all
-
-lemma aux_lt3_high {O : OBdd n m} {U : OBdd n' m'} (O_root_def : O.1.root = .node j) (U_root_def : U.1.root = .node j') (hleq : O.1.heap[j].var.1 < U.1.heap[j'].var.1) :
-    O.1.heap[j].var.1 <
-    min (toVar_or O.1.heap (O.high O_root_def).1.root (max n n'))
+    min (toVar_or O.1.heap O.bdd.heap[j].low (max n n'))
         (toVar_or U.1.heap U.1.root (max n n')) := by
   have := OBdd.var_lt_low_var (h := O_root_def)
   have := OBdd.var_lt_high_var (h := O_root_def)
@@ -344,10 +343,12 @@ lemma aux_lt3_high {O : OBdd n m} {U : OBdd n' m'} (O_root_def : O.1.root = .nod
   simp_all [OBdd.var_eq, toVar_or]
   split <;> simp_all
 
-lemma aux_lt4_low {O : OBdd n m} {U : OBdd n' m'} (O_root_def : O.1.root = .node j) (U_root_def : U.1.root = .node j') (hgeq : O.1.heap[j].var.1 > U.1.heap[j'].var.1) :
-    U.1.heap[j'].var.1 <
-    min (toVar_or O.1.heap O.1.root (max n n'))
-        (toVar_or U.1.heap (U.low U_root_def).1.root (max n n')) := by
+lemma aux_lt3_high {n m n' m' j j'} {O : OBdd n m} {U : OBdd n' m'}
+    (O_root_def : O.1.root = .node j) (U_root_def : U.1.root = .node j')
+    (hleq : O.1.heap[j].var.1 < U.1.heap[j'].var.1) :
+    O.1.heap[j].var.1 <
+    min (toVar_or O.1.heap O.bdd.heap[j].high (max n n'))
+        (toVar_or U.1.heap U.1.root (max n n')) := by
   have := OBdd.var_lt_low_var (h := O_root_def)
   have := OBdd.var_lt_high_var (h := O_root_def)
   have := OBdd.var_lt_low_var (h := U_root_def)
@@ -355,10 +356,12 @@ lemma aux_lt4_low {O : OBdd n m} {U : OBdd n' m'} (O_root_def : O.1.root = .node
   simp_all [OBdd.var_eq, toVar_or]
   split <;> simp_all
 
-lemma aux_lt4_high {O : OBdd n m} {U : OBdd n' m'} (O_root_def : O.1.root = .node j) (U_root_def : U.1.root = .node j') (hgeq : O.1.heap[j].var.1 > U.1.heap[j'].var.1) :
+lemma aux_lt4_low {n m n' m' j j'} {O : OBdd n m} {U : OBdd n' m'}
+    (O_root_def : O.1.root = .node j) (U_root_def : U.1.root = .node j')
+    (hgeq : O.1.heap[j].var.1 > U.1.heap[j'].var.1) :
     U.1.heap[j'].var.1 <
     min (toVar_or O.1.heap O.1.root (max n n'))
-        (toVar_or U.1.heap (U.high U_root_def).1.root (max n n')) := by
+        (toVar_or U.1.heap U.bdd.heap[j'].low (max n n')) := by
   have := OBdd.var_lt_low_var (h := O_root_def)
   have := OBdd.var_lt_high_var (h := O_root_def)
   have := OBdd.var_lt_low_var (h := U_root_def)
@@ -366,10 +369,25 @@ lemma aux_lt4_high {O : OBdd n m} {U : OBdd n' m'} (O_root_def : O.1.root = .nod
   simp_all [OBdd.var_eq, toVar_or]
   split <;> simp_all
 
-lemma aux_lt5_low {O : OBdd n m} {U : OBdd n' m'} (O_root_def : O.1.root = .node j) (U_root_def : U.1.root = .node j') (heeq : O.1.heap[j].var.1 = U.1.heap[j'].var.1) :
+lemma aux_lt4_high {n m n' m' j j'} {O : OBdd n m} {U : OBdd n' m'}
+    (O_root_def : O.1.root = .node j) (U_root_def : U.1.root = .node j')
+    (hgeq : O.1.heap[j].var.1 > U.1.heap[j'].var.1) :
     U.1.heap[j'].var.1 <
-    min (toVar_or O.1.heap (O.low O_root_def).1.root (max n n'))
-        (toVar_or U.1.heap (U.low U_root_def).1.root (max n n')) := by
+    min (toVar_or O.1.heap O.1.root (max n n'))
+        (toVar_or U.1.heap U.bdd.heap[j'].high (max n n')) := by
+  have := OBdd.var_lt_low_var (h := O_root_def)
+  have := OBdd.var_lt_high_var (h := O_root_def)
+  have := OBdd.var_lt_low_var (h := U_root_def)
+  have := OBdd.var_lt_high_var (h := U_root_def)
+  simp_all [OBdd.var_eq, toVar_or]
+  split <;> simp_all
+
+lemma aux_lt5_low {n m n' m' j j'} {O : OBdd n m} {U : OBdd n' m'}
+    (O_root_def : O.1.root = .node j) (U_root_def : U.1.root = .node j')
+    (heeq : O.1.heap[j].var.1 = U.1.heap[j'].var.1) :
+    U.1.heap[j'].var.1 <
+    min (toVar_or O.1.heap O.bdd.heap[j].low (max n n'))
+        (toVar_or U.1.heap U.bdd.heap[j'].low (max n n')) := by
   have h1 := OBdd.var_lt_low_var (h := O_root_def)
   have h2 := OBdd.var_lt_high_var (h := O_root_def)
   have h3 := OBdd.var_lt_low_var (h := U_root_def)
@@ -392,10 +410,12 @@ lemma aux_lt5_low {O : OBdd n m} {U : OBdd n' m'} (O_root_def : O.1.root = .node
       simp_all only [Fin.getElem_fin]
       simp_all
 
-lemma aux_lt5_high {O : OBdd n m} {U : OBdd n' m'} (O_root_def : O.1.root = .node j) (U_root_def : U.1.root = .node j') (heeq : O.1.heap[j].var.1 = U.1.heap[j'].var.1) :
+lemma aux_lt5_high {n m n' m' j j'} {O : OBdd n m} {U : OBdd n' m'}
+    (O_root_def : O.1.root = .node j) (U_root_def : U.1.root = .node j')
+    (heeq : O.1.heap[j].var.1 = U.1.heap[j'].var.1) :
     U.1.heap[j'].var.1 <
-    min (toVar_or O.1.heap (O.high O_root_def).1.root (max n n'))
-        (toVar_or U.1.heap (U.high U_root_def).1.root (max n n')) := by
+    min (toVar_or O.1.heap O.bdd.heap[j].high (max n n'))
+        (toVar_or U.1.heap U.bdd.heap[j'].high (max n n')) := by
   have h2 := OBdd.var_lt_high_var (h := O_root_def)
   have h3 := OBdd.var_lt_low_var (h := U_root_def)
   have h4 := OBdd.var_lt_high_var (h := U_root_def)
@@ -417,789 +437,43 @@ lemma aux_lt5_high {O : OBdd n m} {U : OBdd n' m'} (O_root_def : O.1.root = .nod
       simp_all only [Fin.getElem_fin]
       simp_all
 
-def apply_helper (op : (Bool → Bool → Bool)) (O : OBdd n m) (U : OBdd n' m') (s0 : State n n' m m') (inv : Invariant op O U s0) :
-    { r : State n n' m m' × RawPointer //
-      (Invariant op O U r.1) ∧
-      (r.1.cache[(⟨O.1.root, U.1.root⟩ : Pointer m × Pointer m')]? = some r.2) ∧
-      (s0.size ≤ r.1.size) ∧
-      (∀ (k : Pointer m × Pointer m'),
-        (∀ p, s0.cache[k]? = some p → r.1.cache[k]? = some p) ∧
-        (r.1.cache[k]? = none → s0.cache[k]? = none) ∧
-        (s0.cache[k]? = none → (∃ p, r.1.cache[k]? = some p) → Pointer.Reachable O.1.heap O.1.root k.1 ∧ Pointer.Reachable U.1.heap U.1.root k.2))
-    } :=
+def apply_helper {n m n' m'} (op : (Bool → Bool → Bool)) (O : OBdd n m) (U : OBdd n' m')
+    (s0 : State n n' m m') :
+    State n n' m m' × RawPointer :=
   match hc : cache_get O.1.root U.1.root s0 with
-  | some root => ⟨⟨s0, root⟩, ⟨inv, hc, .refl, by grind only⟩⟩
+  | some root => ⟨s0, root⟩
   | none =>
     match O_root_def : O.1.root with
     | .terminal b =>
       match U_root_def : U.1.root with
       | .terminal b' =>
-        ⟨⟨⟨s0.size, s0.heap, s0.cache.insert ⟨O.1.root, U.1.root⟩ (.inl (op b b'))⟩, .inl (op b b')⟩, by
-          constructor
-          · exact insert_terminal_invariant s0 inv O_root_def U_root_def
-          · constructor
-            · simp only [O_root_def, U_root_def, Std.HashMap.getElem?_insert_self]
-            · constructor
-              · exact .refl
-              ·
-                intro k
-                constructor
-                · intro p hp
-                  simp only [cache_get] at hc
-                  rw [← hp]
-                  simp only [Std.HashMap.getElem?_insert, beq_iff_eq, ite_eq_right_iff]
-                  intro contra
-                  subst contra
-                  rw [hc] at hp
-                  contradiction
-                · constructor
-                  · simp only [getElem?_eq_none_iff, Std.HashMap.mem_insert, beq_iff_eq, not_or,
-                      and_imp, imp_self, implies_true]
-                  · rintro h1 ⟨p, hp⟩
-                    simp only [Std.HashMap.getElem?_insert,beq_iff_eq] at hp
-                    split at hp
-                    next heq =>
-                      subst heq
-                      simp only [O_root_def, Pointer.Reachable.refl, U_root_def, and_self]
-                    next heq => rw [h1] at hp; contradiction
-        ⟩
+        ⟨⟨s0.size, s0.heap, s0.cache.insert ⟨O.1.root, U.1.root⟩ (.inl (op b b'))⟩, .inl (op b b')⟩
       | .node j' =>
-        let ⟨⟨sl, rl⟩, ⟨invl, hl, hsl, hlp⟩⟩ := apply_helper op O (U.low U_root_def) s0 inv
-        let ⟨⟨sh, rh⟩, ⟨invh, hh, hsh, hhp⟩⟩ := apply_helper op O (U.high U_root_def) sl invl
-        let ⟨r, ⟨invv, hv, hsv, hvp⟩⟩ :=
-          heap_push (O := O) (U := U)
-            ⟨⟨U.1.heap[j'].var.1, by omega⟩, rl, rh⟩ sh invh
-            (by
-              use ⟨O.1.root, ((U.low U_root_def).1.root)⟩
-              simp only
-              exact (hhp _).1 _ hl
-            )
-            ⟨_, hh⟩
-            (by
-              simp only
-              rw [O_root_def, U_root_def]
-              simp only [Fin.getElem_fin, toVar_or, le_sup_iff, Fin.is_le', or_true,
-                inf_of_le_right]
-            )
-            (by
-              intro j hj1
-              simp only [Fin.getElem_fin]
-              intro hj2
-              have := (hhp _).1 _ hl
-              simp only at this
-              rw [hj2] at this
-              have that := (invh.2 _ (.inr j) this).1 _ hj1 rfl
-              simp only at that
-              rw [that]
-              exact aux_lt1_low O_root_def U_root_def
-            )
-            (by
-              intro j hj1
-              simp only [Fin.getElem_fin]
-              intro hj2
-              have := (invh.2 _ _ hh).1 _ hj1 hj2
-              rw [this]
-              exact aux_lt1_high O_root_def U_root_def
-            )
-            (by
-              intro h0 h1 I
-              symm
-              simp only [OBdd.evaluate_node U_root_def, OBdd.evaluate_terminal O_root_def]
-              rw [op_if1 op]
-              simp only [Nat.sub_zero, Fin.getElem_fin, Vector.getElem_cast, cook_heap,
-                RawNode.cook, Pointer.node.injEq, OBdd.evaluate_node, Vector.getElem_ofFn,
-                Vector.getElem_push_eq]
-              congr 1
-              · have := Vector.getElem_extract (as := I) (start := 0) (stop := n') (i := U.1.heap[j'.1].var.1) (by omega)
-                simp only [this, zero_add]
-              · conv =>
-                  rhs
-                  congr
-                  congr
-                  congr
-                  rfl
-                  simp [cook_heap, RawNode.cook]
-                  rfl
-                symm
-                have h := invh.2 ⟨O.1.root, (U.high U_root_def).1.root⟩ rh hh
-                rcases h with ⟨h1, h2, h3, h4, h5, h6⟩
-                rw [O.evaluate_terminal (by simp [O_root_def]; rfl)] at h6
-                rw [push_evaluate rfl (h0 := h0) (ho := h5)]
-                · exact h6 I
-                · simp only [OBdd.high_root_eq_high, Fin.getElem_fin, Vector.getElem_ofFn,
-                    Vector.getElem_push_eq]
-                · grind only [RawPointer.Bounded]
-              · conv =>
-                  rhs
-                  congr
-                  congr
-                  congr
-                  rfl
-                  simp [cook_heap, RawNode.cook]
-                  rfl
-                symm
-                have : sh.cache[(⟨O.1.root, (U.low U_root_def).1.root⟩ : Pointer m × Pointer m')]? = some rl := by
-                  apply (hhp _).1
-                  exact hl
-                have h := invh.2 ⟨O.1.root, (U.low U_root_def).1.root⟩ rl this
-                rcases h with ⟨h1, h2, h3, h4, h5, h6⟩
-                simp only [OBdd.mk_eq_self, Vector.take_eq_extract, O.evaluate_terminal O_root_def,
-                  OBdd.high_heap_eq_heap, OBdd.low_root_eq_low, U.mk_eq_low U_root_def] at h6
-                rw [push_evaluate rfl (h0 := h0) (ho := h5)]
-                · exact h6 I
-                · simp only [OBdd.low_root_eq_low, Fin.getElem_fin, Vector.getElem_ofFn,
-                    Vector.getElem_push_eq]
-                · grind only [RawPointer.Bounded]
-            )
-            (by
-              simp only [cache_get] at hc
-              cases heq : sh.cache[(⟨O.1.root, U.1.root⟩ : Pointer m × Pointer m')]? with
-              | none => rfl
-              | some val =>
-                cases heqq : sl.cache[(⟨O.1.root, U.1.root⟩ : Pointer m × Pointer m')]? with
-                | none =>
-                  have := ((hhp _).2.2 heqq ⟨val, heq⟩).2
-                  simp only [OBdd.high_heap_eq_heap] at this
-                  absurd this
-                  apply OBdd.not_oedge_reachable
-                  exact oedge_of_high
-                | some val =>
-                  have := ((hlp _).2.2 hc ⟨_, heqq⟩).2
-                  simp only [OBdd.low_heap_eq_heap] at this
-                  absurd this
-                  apply OBdd.not_oedge_reachable
-                  exact oedge_of_low
-            )
-        ⟨ r,
-          invv,
-          (by rw [O_root_def, U_root_def] at hv; exact hv),
-          .trans hsl (.trans hsh hsv),
-          by
-            intro k
-            constructor
-            · intro p hp
-              apply (hvp _).1
-              apply (hhp _).1
-              apply (hlp _).1
-              exact hp
-            · constructor
-              · intro hk
-                apply (hlp _).2.1
-                apply (hhp _).2.1
-                apply (hvp _).2.1
-                exact hk
-              · intro hk hkp
-                rw [← O_root_def, ← U_root_def]
-                cases heq : sh.cache[k]? with
-                | none =>
-                  apply (hvp _).2.2 heq hkp
-                | some w =>
-                  cases heqq : sl.cache[k]? with
-                  | none =>
-                    have := (hhp _).2.2 heqq ⟨_, heq⟩
-                    rw [OBdd.high_heap_eq_heap, OBdd.high_root_eq_high] at this
-                    constructor
-                    · exact this.1
-                    · exact .trans (U.bdd.reachable_high U_root_def) this.2
-                  | some ww =>
-                    have := (hlp _).2.2 hk ⟨_, heqq⟩
-                    rw [OBdd.low_heap_eq_heap, OBdd.low_root_eq_low] at this
-                    constructor
-                    · exact this.1
-                    · exact .trans (U.bdd.reachable_low U_root_def) this.2
-        ⟩
+        let ⟨sl, rl⟩ := apply_helper op O (U.low U_root_def) s0
+        let ⟨sh, rh⟩ := apply_helper op O (U.high U_root_def) sl
+        heap_push O U ⟨⟨U.1.heap[j'].var.1, by omega⟩, rl, rh⟩ sh
     | .node j =>
       match U_root_def : U.1.root with
       | .terminal b' =>
-        let ⟨⟨sl, rl⟩, ⟨invl, hl, hsl, hlp⟩⟩ := apply_helper op (O.low O_root_def) U s0 inv
-        let ⟨⟨sh, rh⟩, ⟨invh, hh, hsh, hhp⟩⟩ := apply_helper op (O.high O_root_def) U sl invl
-        let ⟨r, ⟨invv, hv, hsv, hvp⟩⟩ :=
-          heap_push (O := O) (U := U)
-            ⟨⟨O.1.heap[j].var.1, by omega⟩, rl, rh⟩ sh invh
-            ⟨_, (hhp _).1 _ hl⟩
-            ⟨_, hh⟩
-            (by
-              simp only
-              rw [O_root_def, U_root_def]
-              simp only [Fin.getElem_fin, toVar_or, le_sup_iff, Fin.is_le', true_or, inf_of_le_left]
-            )
-            (by
-              intro j hj1
-              simp only [Fin.getElem_fin]
-              intro hj2
-              have := (hhp _).1 _ hl
-              simp only at this
-              rw [hj2] at this
-              have that := (invh.2 _ (.inr j) this).1 _ hj1 rfl
-              simp only at that
-              rw [that]
-              exact aux_lt2_low O_root_def U_root_def
-            )
-            (by
-              intro j hj1
-              simp only [Fin.getElem_fin]
-              intro hj2
-              have := (invh.2 _ _ hh).1 _ hj1 hj2
-              rw [this]
-              exact aux_lt2_high O_root_def U_root_def
-            )
-            (by
-              intro h0 h1 I
-              symm
-              simp only [OBdd.evaluate_node O_root_def, OBdd.evaluate_terminal U_root_def]
-              rw [op_if2 op]
-              simp only [Nat.sub_zero, Fin.getElem_fin, Vector.getElem_cast, cook_heap,
-                RawNode.cook, Pointer.node.injEq, OBdd.evaluate_node, Vector.getElem_ofFn,
-                Vector.getElem_push_eq]
-              congr 1
-              · have := Vector.getElem_extract (as := I) (start := 0) (stop := n) (i := O.1.heap[j.1].var.1) (by omega)
-                simp only [zero_add, this]
-              · conv =>
-                  rhs
-                  congr
-                  congr
-                  congr
-                  rfl
-                  simp [cook_heap, RawNode.cook]
-                  rfl
-                symm
-                have h := invh.2 ⟨(O.high O_root_def).1.root, U.1.root⟩ rh hh
-                rcases h with ⟨h1, h2, h3, h4, h5, h6⟩
-                simp only [OBdd.high_heap_eq_heap, OBdd.high_root_eq_high, O.mk_eq_high O_root_def,
-                  Vector.take_eq_extract, OBdd.mk_eq_self, U.evaluate_terminal U_root_def] at h6
-                rw [push_evaluate rfl (h0 := h0) (ho := h5)]
-                · exact h6 I
-                · simp only [OBdd.high_root_eq_high, Fin.getElem_fin, Vector.getElem_ofFn,
-                    Vector.getElem_push_eq]
-                · grind only [RawPointer.Bounded]
-              · conv =>
-                  rhs
-                  congr
-                  congr
-                  congr
-                  rfl
-                  simp [cook_heap, RawNode.cook]
-                  rfl
-                symm
-                have : sh.cache[(⟨(O.low O_root_def).1.root, U.1.root⟩ : Pointer m × Pointer m')]? = some rl := by
-                  apply (hhp _).1
-                  exact hl
-                have h := invh.2 ⟨(O.low O_root_def).1.root, U.1.root⟩ rl this
-                rcases h with ⟨h1, h2, h3, h4, h5, h6⟩
-                simp only [OBdd.high_heap_eq_heap, Vector.take_eq_extract, OBdd.mk_eq_self,
-                  U.evaluate_terminal U_root_def] at h6
-                rw [push_evaluate rfl (h0 := h0) (ho := h5)]
-                · exact h6 I
-                · simp only [OBdd.low_root_eq_low, Fin.getElem_fin, Vector.getElem_ofFn,
-                    Vector.getElem_push_eq]
-                · grind only [RawPointer.Bounded]
-            )
-            (by
-              simp only [cache_get] at hc
-              cases heq : sh.cache[(⟨O.1.root, U.1.root⟩ : Pointer m × Pointer m')]? with
-              | none => rfl
-              | some val =>
-                cases heqq : sl.cache[(⟨O.1.root, U.1.root⟩ : Pointer m × Pointer m')]? with
-                | none =>
-                  have := ((hhp _).2.2 heqq ⟨val, heq⟩).1
-                  simp only [OBdd.high_heap_eq_heap] at this
-                  absurd this
-                  apply OBdd.not_oedge_reachable
-                  exact oedge_of_high
-                | some val =>
-                  have := ((hlp _).2.2 hc ⟨_, heqq⟩).1
-                  simp only [OBdd.low_heap_eq_heap] at this
-                  absurd this
-                  apply OBdd.not_oedge_reachable
-                  exact oedge_of_low
-            )
-        ⟨ r,
-          invv,
-          (by rw [O_root_def, U_root_def] at hv; exact hv),
-          .trans hsl (.trans hsh hsv),
-          by
-            intro k
-            constructor
-            · intro p hp
-              apply (hvp _).1
-              apply (hhp _).1
-              apply (hlp _).1
-              exact hp
-            · constructor
-              · intro hk
-                apply (hlp _).2.1
-                apply (hhp _).2.1
-                apply (hvp _).2.1
-                exact hk
-              · intro hk hkp
-                rw [← O_root_def, ← U_root_def]
-                cases heq : sh.cache[k]? with
-                | none =>
-                  apply (hvp _).2.2 heq hkp
-                | some w =>
-                  cases heqq : sl.cache[k]? with
-                  | none =>
-                    have := (hhp _).2.2 heqq ⟨_, heq⟩
-                    rw [OBdd.high_heap_eq_heap, OBdd.high_root_eq_high] at this
-                    constructor
-                    · exact .trans (O.bdd.reachable_high O_root_def) this.1
-                    · exact this.2
-                  | some ww =>
-                    have := (hlp _).2.2 hk ⟨_, heqq⟩
-                    rw [OBdd.low_heap_eq_heap, OBdd.low_root_eq_low] at this
-                    constructor
-                    · exact .trans (O.bdd.reachable_low O_root_def) this.1
-                    · exact this.2
-        ⟩
+        let ⟨sl, rl⟩ := apply_helper op (O.low O_root_def) U s0
+        let ⟨sh, rh⟩ := apply_helper op (O.high O_root_def) U sl
+        heap_push O U ⟨⟨O.1.heap[j].var.1, by omega⟩, rl, rh⟩ sh
       | .node j' =>
         if hlt : O.1.heap[j].var.1 < U.1.heap[j'].var.1
         then
-          let ⟨⟨sl, rl⟩, ⟨invl, hl, hsl, hlp⟩⟩ := apply_helper op (O.low O_root_def) U s0 inv
-          let ⟨⟨sh, rh⟩, ⟨invh, hh, hsh, hhp⟩⟩ := apply_helper op (O.high O_root_def) U sl invl
-          let ⟨r, ⟨invv, hv, hsv, hvp⟩⟩ :=
-            heap_push (O := O) (U := U)
-              ⟨⟨O.1.heap[j].var.1, by omega⟩, rl, rh⟩ sh invh
-              ⟨_, (hhp _).1 _ hl⟩
-              ⟨_, hh⟩
-              (by
-                simp only
-                rw [O_root_def, U_root_def]
-                simp only [Fin.getElem_fin, toVar_or]
-                exact Eq.symm (min_eq_left_of_lt hlt)
-              )
-              (by
-                intro j'' hj1
-                simp only [Fin.getElem_fin]
-                intro hj2
-                have := (hhp _).1 _ hl
-                simp only at this
-                rw [hj2] at this
-                have that := (invh.2 _ _ this).1 _ hj1 rfl
-                simp only at that
-                rw [that]
-                exact aux_lt3_low O_root_def U_root_def hlt
-              )
-              (by
-                intro j'' hj1
-                simp only [Fin.getElem_fin]
-                intro hj2
-                have := (invh.2 _ _ hh).1 _ hj1 hj2
-                rw [this]
-                exact aux_lt3_high O_root_def U_root_def hlt
-              )
-              (by
-                intro h0 h1 I
-                symm
-                simp only [OBdd.evaluate_node O_root_def, OBdd.evaluate_node U_root_def]
-                rw [op_if2 op]
-                simp only [Nat.sub_zero, Fin.getElem_fin, Vector.getElem_cast, cook_heap,
-                  RawNode.cook, Pointer.node.injEq, OBdd.evaluate_node, Vector.getElem_ofFn,
-                  Vector.getElem_push_eq]
-                congr 1
-                · have := Vector.getElem_extract (as := I) (start := 0) (stop := n) (i := O.1.heap[j.1].var.1) (by omega)
-                  simp only [this, zero_add]
-                · conv =>
-                    rhs
-                    congr
-                    congr
-                    congr
-                    rfl
-                    simp [cook_heap, RawNode.cook]
-                    rfl
-                  symm
-                  have h := invh.2 ⟨(O.high O_root_def).1.root, U.1.root⟩ rh hh
-                  rcases h with ⟨h1, h2, h3, h4, h5, h6⟩
-                  simp only [OBdd.high_heap_eq_heap, OBdd.high_root_eq_high, O.mk_eq_high O_root_def,
-                    Vector.take_eq_extract, OBdd.mk_eq_self] at h6
-                  rw [push_evaluate rfl (h0 := h0) (ho := h5)]
-                  · simp_all only [Fin.getElem_fin, Pointer.node.injEq, OBdd.evaluate_node,
-                      Vector.getElem_cast]
-                  · simp only [OBdd.high_root_eq_high, Fin.getElem_fin, Vector.getElem_ofFn,
-                      Vector.getElem_push_eq]
-                  · grind only [RawPointer.Bounded]
-                · conv =>
-                    rhs
-                    congr
-                    congr
-                    congr
-                    rfl
-                    simp [cook_heap, RawNode.cook]
-                    rfl
-                  symm
-                  have : sh.cache[(⟨(O.low O_root_def).1.root, U.1.root⟩ : Pointer m × Pointer m')]? = some rl := by
-                    apply (hhp _).1
-                    exact hl
-                  have h := invh.2 ⟨(O.low O_root_def).1.root, U.1.root⟩ rl this
-                  rcases h with ⟨h1, h2, h3, h4, h5, h6⟩
-                  simp only [OBdd.high_heap_eq_heap, OBdd.low_root_eq_low, O.mk_eq_low O_root_def,
-                    Vector.take_eq_extract, OBdd.mk_eq_self] at h6
-                  rw [push_evaluate rfl (h0 := h0) (ho := h5)]
-                  · simp_all only [Fin.getElem_fin, Pointer.node.injEq, OBdd.evaluate_node,
-                      Vector.getElem_cast]
-                  · simp only [OBdd.low_root_eq_low, Fin.getElem_fin, Vector.getElem_ofFn,
-                      Vector.getElem_push_eq]
-                  · grind only [RawPointer.Bounded]
-              )
-              (by
-                simp only [cache_get] at hc
-                cases heq : sh.cache[(⟨O.1.root, U.1.root⟩ : Pointer m × Pointer m')]? with
-                | none => rfl
-                | some val =>
-                  cases heqq : sl.cache[(⟨O.1.root, U.1.root⟩ : Pointer m × Pointer m')]? with
-                  | none =>
-                    have := ((hhp _).2.2 heqq ⟨val, heq⟩).1
-                    simp only [OBdd.high_heap_eq_heap] at this
-                    absurd this
-                    apply OBdd.not_oedge_reachable
-                    exact oedge_of_high
-                  | some val =>
-                    have := ((hlp _).2.2 hc ⟨_, heqq⟩).1
-                    simp only [OBdd.low_heap_eq_heap] at this
-                    absurd this
-                    apply OBdd.not_oedge_reachable
-                    exact oedge_of_low
-              )
-          ⟨ r,
-            invv,
-            (by rw [O_root_def, U_root_def] at hv; exact hv),
-            .trans hsl (.trans hsh hsv),
-            by
-              intro k
-              constructor
-              · intro p hp
-                apply (hvp _).1
-                apply (hhp _).1
-                apply (hlp _).1
-                exact hp
-              · constructor
-                · intro hk
-                  apply (hlp _).2.1
-                  apply (hhp _).2.1
-                  apply (hvp _).2.1
-                  exact hk
-                · intro hk hkp
-                  rw [← O_root_def, ← U_root_def]
-                  cases heq : sh.cache[k]? with
-                  | none =>
-                    apply (hvp _).2.2 heq hkp
-                  | some w =>
-                    cases heqq : sl.cache[k]? with
-                    | none =>
-                      have := (hhp _).2.2 heqq ⟨_, heq⟩
-                      rw [OBdd.high_heap_eq_heap, OBdd.high_root_eq_high] at this
-                      constructor
-                      · exact .trans (O.bdd.reachable_high O_root_def) this.1
-                      · exact this.2
-                    | some ww =>
-                      have := (hlp _).2.2 hk ⟨_, heqq⟩
-                      rw [OBdd.low_heap_eq_heap, OBdd.low_root_eq_low] at this
-                      constructor
-                      · exact .trans (O.bdd.reachable_low O_root_def) this.1
-                      · exact this.2
-          ⟩
+          let ⟨sl, rl⟩ := apply_helper op (O.low O_root_def) U s0
+          let ⟨sh, rh⟩ := apply_helper op (O.high O_root_def) U sl
+          heap_push O U ⟨⟨O.1.heap[j].var.1, by omega⟩, rl, rh⟩ sh
         else
           if hgeq : O.1.heap[j].var.1 > U.1.heap[j'].var.1
           then
-            let ⟨⟨sl, rl⟩, ⟨invl, hl, hsl, hlp⟩⟩ := apply_helper op O (U.low U_root_def) s0 inv
-            let ⟨⟨sh, rh⟩, ⟨invh, hh, hsh, hhp⟩⟩ := apply_helper op O (U.high U_root_def) sl invl
-            let ⟨r, ⟨invv, hv, hsv, hvp⟩⟩ :=
-              heap_push (O := O) (U := U)
-                ⟨⟨U.1.heap[j'].var.1, by omega⟩, rl, rh⟩ sh invh
-                ⟨_, (hhp _).1 _ hl⟩
-                ⟨_, hh⟩
-                (by
-                  simp only
-                  rw [O_root_def, U_root_def]
-                  simp only [Fin.getElem_fin, toVar_or]
-                  exact Eq.symm (min_eq_right_of_lt hgeq)
-                )
-                (by
-                  intro j'' hj1
-                  simp only [Fin.getElem_fin]
-                  intro hj2
-                  have := (hhp _).1 _ hl
-                  simp only at this
-                  rw [hj2] at this
-                  have that := (invh.2 _ _ this).1 _ hj1 rfl
-                  simp only at that
-                  rw [that]
-                  exact aux_lt4_low O_root_def U_root_def hgeq
-                )
-                (by
-                  intro j'' hj1
-                  simp only [Fin.getElem_fin]
-                  intro hj2
-                  have := (invh.2 _ _ hh).1 _ hj1 hj2
-                  rw [this]
-                  exact aux_lt4_high O_root_def U_root_def hgeq
-                )
-                (by
-                  intro h0 h1 I
-                  symm
-                  simp only [OBdd.evaluate_node O_root_def, OBdd.evaluate_node U_root_def]
-                  rw [op_if1 op]
-                  simp only [Nat.sub_zero, Fin.getElem_fin, Vector.getElem_cast, cook_heap,
-                    RawNode.cook, Pointer.node.injEq, OBdd.evaluate_node, Vector.getElem_ofFn,
-                    Vector.getElem_push_eq]
-                  congr 1
-                  · have := Vector.getElem_extract (as := I) (start := 0) (stop := n') (i := U.1.heap[j'.1].var.1) (by omega)
-                    simp only [this, zero_add]
-                  · conv =>
-                      rhs
-                      congr
-                      congr
-                      congr
-                      rfl
-                      simp [cook_heap, RawNode.cook]
-                      rfl
-                    symm
-                    have h := invh.2 ⟨O.1.root, (U.high U_root_def).1.root⟩ rh hh
-                    rcases h with ⟨h1, h2, h3, h4, h5, h6⟩
-                    simp only [OBdd.mk_eq_self, Vector.take_eq_extract, OBdd.high_heap_eq_heap,
-                      OBdd.high_root_eq_high, U.mk_eq_high U_root_def] at h6
-                    rw [push_evaluate rfl (h0 := h0) (ho := h5)]
-                    · simp_all only [Fin.getElem_fin, Pointer.node.injEq, OBdd.evaluate_node,
-                        Vector.getElem_cast]
-                    · simp only [OBdd.high_root_eq_high, Fin.getElem_fin, Vector.getElem_ofFn,
-                        Vector.getElem_push_eq]
-                    · grind only [RawPointer.Bounded]
-                  · conv =>
-                      rhs
-                      congr
-                      congr
-                      congr
-                      rfl
-                      simp [cook_heap, RawNode.cook]
-                      rfl
-                    symm
-                    have : sh.cache[(⟨O.1.root, (U.low U_root_def).1.root⟩ : Pointer m × Pointer m')]? = some rl := by
-                      apply (hhp _).1
-                      exact hl
-                    have h := invh.2 ⟨O.1.root, (U.low U_root_def).1.root⟩ rl this
-                    rcases h with ⟨h1, h2, h3, h4, h5, h6⟩
-                    simp only [OBdd.mk_eq_self, Vector.take_eq_extract, OBdd.high_heap_eq_heap,
-                      OBdd.low_root_eq_low, U.mk_eq_low U_root_def] at h6
-                    rw [push_evaluate rfl (h0 := h0) (ho := h5)]
-                    · simp_all only [Fin.getElem_fin, Pointer.node.injEq, OBdd.evaluate_node,
-                        Vector.getElem_cast]
-                    · simp only [OBdd.low_root_eq_low, Fin.getElem_fin, Vector.getElem_ofFn,
-                        Vector.getElem_push_eq]
-                    · grind only [RawPointer.Bounded]
-                )
-                (by
-                  simp only [cache_get] at hc
-                  cases heq : sh.cache[(⟨O.1.root, U.1.root⟩ : Pointer m × Pointer m')]? with
-                  | none => rfl
-                  | some val =>
-                    cases heqq : sl.cache[(⟨O.1.root, U.1.root⟩ : Pointer m × Pointer m')]? with
-                    | none =>
-                      have := ((hhp _).2.2 heqq ⟨val, heq⟩).2
-                      simp only [OBdd.high_heap_eq_heap] at this
-                      absurd this
-                      apply OBdd.not_oedge_reachable
-                      exact oedge_of_high
-                    | some val =>
-                      have := ((hlp _).2.2 hc ⟨_, heqq⟩).2
-                      simp only [OBdd.low_heap_eq_heap] at this
-                      absurd this
-                      apply OBdd.not_oedge_reachable
-                      exact oedge_of_low
-                )
-            ⟨ r,
-              invv,
-              (by rw [O_root_def, U_root_def] at hv; exact hv),
-              .trans hsl (.trans hsh hsv),
-              by
-                intro k
-                constructor
-                · intro p hp
-                  apply (hvp _).1
-                  apply (hhp _).1
-                  apply (hlp _).1
-                  exact hp
-                · constructor
-                  · intro hk
-                    apply (hlp _).2.1
-                    apply (hhp _).2.1
-                    apply (hvp _).2.1
-                    exact hk
-                  · intro hk hkp
-                    rw [← O_root_def, ← U_root_def]
-                    cases heq : sh.cache[k]? with
-                    | none =>
-                      apply (hvp _).2.2 heq hkp
-                    | some w =>
-                      cases heqq : sl.cache[k]? with
-                      | none =>
-                        have := (hhp _).2.2 heqq ⟨_, heq⟩
-                        rw [OBdd.high_heap_eq_heap, OBdd.high_root_eq_high] at this
-                        constructor
-                        · exact this.1
-                        · exact .trans (U.bdd.reachable_high U_root_def) this.2
-                      | some ww =>
-                        have := (hlp _).2.2 hk ⟨_, heqq⟩
-                        rw [OBdd.low_heap_eq_heap, OBdd.low_root_eq_low] at this
-                        constructor
-                        · exact this.1
-                        · exact .trans (U.bdd.reachable_low U_root_def) this.2
-            ⟩
+            let ⟨sl, rl⟩ := apply_helper op O (U.low U_root_def) s0
+            let ⟨sh, rh⟩ := apply_helper op O (U.high U_root_def) sl
+            heap_push O U ⟨⟨U.1.heap[j'].var.1, by omega⟩, rl, rh⟩ sh
           else
-            let ⟨⟨sl, rl⟩, ⟨invl, hl, hsl, hlp⟩⟩ := apply_helper op (O.low O_root_def) (U.low U_root_def) s0 inv
-            let ⟨⟨sh, rh⟩, ⟨invh, hh, hsh, hhp⟩⟩ := apply_helper op (O.high O_root_def) (U.high U_root_def) sl invl
-            let ⟨r, ⟨invv, hv, hsv, hvp⟩⟩ :=
-              heap_push (O := O) (U := U)
-                ⟨⟨U.1.heap[j'].var.1, by omega⟩, rl, rh⟩ sh invh
-                ⟨_, (hhp _).1 _ hl⟩
-                ⟨_, hh⟩
-                (by
-                  simp only
-                  rw [O_root_def, U_root_def]
-                  simp only [Fin.getElem_fin, toVar_or]
-                  have heeq : O.1.heap[j].var.1 = U.1.heap[j'].var.1 := by omega
-                  simp only [Fin.getElem_fin] at heeq
-                  rw [heeq]
-                  simp only [min_self]
-                )
-                (by
-                  intro j'' hj1
-                  simp only [Fin.getElem_fin]
-                  intro hj2
-                  have := (hhp _).1 _ hl
-                  simp only at this
-                  rw [hj2] at this
-                  have that := (invh.2 _ _ this).1 _ hj1 rfl
-                  simp only at that
-                  rw [that]
-                  exact aux_lt5_low O_root_def U_root_def (by omega)
-                )
-                (by
-                  intro j'' hj1
-                  simp only [Fin.getElem_fin]
-                  intro hj2
-                  have := (invh.2 _ _ hh).1 _ hj1 hj2
-                  rw [this]
-                  exact aux_lt5_high O_root_def U_root_def (by omega)
-                )
-                (by
-                  intro h0 h1 I
-                  symm
-                  simp only [OBdd.evaluate_node U_root_def, OBdd.evaluate_node O_root_def]
-                  have heeq : O.1.heap[j].var.1 = U.1.heap[j'].var.1 := by omega
-                  have heo := Vector.getElem_extract (as := I) (start := 0) (stop := n) (i := O.1.heap[j.1].var.1) (by omega)
-                  have heu := Vector.getElem_extract (as := I) (start := 0) (stop := n') (i := U.1.heap[j'.1].var.1) (by omega)
-                  have : (Vector.cast (m := n') (by omega) (I.extract 0 n'))[U.1.heap[j'].var] = (Vector.cast (m := n) (by omega) (I.extract 0 n))[O.1.heap[j].var] := by
-                    simp only [Fin.getElem_fin]
-                    rw [Vector.getElem_cast]
-                    rw [Vector.getElem_cast]
-                    rw [heo]
-                    rw [heu]
-                    simp only [zero_add]
-                    congr 1
-                    symm
-                    exact heeq
-                  rw [this]
-                  rw [op_if3 op]
-                  simp only [Nat.sub_zero, Fin.getElem_fin, Vector.getElem_cast, cook_heap,
-                    RawNode.cook, Pointer.node.injEq, OBdd.evaluate_node, Vector.getElem_ofFn,
-                    Vector.getElem_push_eq]
-                  congr 1
-                  · simp only [zero_add] at heo
-                    simp_all only [getElem?_eq_none_iff, OBdd.low_heap_eq_heap, forall_exists_index,
-                      Prod.forall, OBdd.high_heap_eq_heap, Fin.getElem_fin, Nat.sub_zero, zero_add,
-                      Vector.getElem_cast]
-                  · conv =>
-                      rhs
-                      congr
-                      congr
-                      congr
-                      rfl
-                      simp [cook_heap, RawNode.cook]
-                      rfl
-                    symm
-                    have h := invh.2 ⟨(O.high O_root_def).1.root, (U.high U_root_def).1.root⟩ rh hh
-                    rcases h with ⟨h1, h2, h3, h4, h5, h6⟩
-                    rw [push_evaluate rfl (h0 := h0) (ho := h5)]
-                    · exact h6 I
-                    · simp only [OBdd.high_root_eq_high, Fin.getElem_fin, Vector.getElem_ofFn,
-                        Vector.getElem_push_eq]
-                    · grind only [RawPointer.Bounded]
-                  · conv =>
-                      rhs
-                      congr
-                      congr
-                      congr
-                      rfl
-                      simp [cook_heap, RawNode.cook]
-                      rfl
-                    symm
-                    have : sh.cache[(⟨(O.low O_root_def).1.root, (U.low U_root_def).1.root⟩ : Pointer m × Pointer m')]? = some rl := by
-                      apply (hhp _).1
-                      exact hl
-                    have h := invh.2 ⟨(O.low O_root_def).1.root, (U.low U_root_def).1.root⟩ rl this
-                    rcases h with ⟨h1, h2, h3, h4, h5, h6⟩
-                    rw [push_evaluate rfl (h0 := h0) (ho := h5)]
-                    · exact h6 I
-                    · simp only [OBdd.low_root_eq_low, Fin.getElem_fin, Vector.getElem_ofFn,
-                        Vector.getElem_push_eq]
-                    · grind only [RawPointer.Bounded]
-                )
-                (by
-                  simp only [cache_get] at hc
-                  cases heq : sh.cache[(⟨O.1.root, U.1.root⟩ : Pointer m × Pointer m')]? with
-                  | none => rfl
-                  | some val =>
-                    cases heqq : sl.cache[(⟨O.1.root, U.1.root⟩ : Pointer m × Pointer m')]? with
-                    | none =>
-                      have := ((hhp _).2.2 heqq ⟨val, heq⟩).2
-                      simp only [OBdd.high_heap_eq_heap] at this
-                      absurd this
-                      apply OBdd.not_oedge_reachable
-                      exact oedge_of_high
-                    | some val =>
-                      have := ((hlp _).2.2 hc ⟨_, heqq⟩).2
-                      simp only [OBdd.low_heap_eq_heap] at this
-                      absurd this
-                      apply OBdd.not_oedge_reachable
-                      exact oedge_of_low
-                )
-          ⟨ r,
-            invv,
-            (by rw [O_root_def, U_root_def] at hv; exact hv),
-            .trans hsl (.trans hsh hsv),
-            by
-              intro k
-              constructor
-              · intro p hp
-                apply (hvp _).1
-                apply (hhp _).1
-                apply (hlp _).1
-                exact hp
-              · constructor
-                · intro hk
-                  apply (hlp _).2.1
-                  apply (hhp _).2.1
-                  apply (hvp _).2.1
-                  exact hk
-                · intro hk hkp
-                  rw [← O_root_def, ← U_root_def]
-                  cases heq : sh.cache[k]? with
-                  | none =>
-                    apply (hvp _).2.2 heq hkp
-                  | some w =>
-                    cases heqq : sl.cache[k]? with
-                    | none =>
-                      have := (hhp _).2.2 heqq ⟨_, heq⟩
-                      simp only [OBdd.high_heap_eq_heap, OBdd.high_root_eq_high] at this
-                      constructor
-                      · exact .trans (O.bdd.reachable_high O_root_def) this.1
-                      · exact .trans (U.bdd.reachable_high U_root_def) this.2
-                    | some ww =>
-                      have := (hlp _).2.2 hk ⟨_, heqq⟩
-                      simp only [OBdd.low_heap_eq_heap, OBdd.low_root_eq_low] at this
-                      constructor
-                      · exact .trans (O.bdd.reachable_low O_root_def) this.1
-                      · exact .trans (U.bdd.reachable_low U_root_def) this.2
-          ⟩
+            let ⟨sl, rl⟩ := apply_helper op (O.low O_root_def) (U.low U_root_def) s0
+            let ⟨sh, rh⟩ := apply_helper op (O.high O_root_def) (U.high U_root_def) sl
+           heap_push O U ⟨⟨U.1.heap[j'].var.1, by omega⟩, rl, rh⟩ sh
 termination_by (O, U)
 decreasing_by
   · right; exact oedge_of_low
@@ -1213,21 +487,729 @@ decreasing_by
   · left; exact oedge_of_low
   · left; exact oedge_of_high
 
-public def oapply (op : Bool → Bool → Bool) (O : OBdd n m) (U : OBdd n' m') :
-    (s : Nat) ×
-    { OU : OBdd (n ⊔ n') s //
-      ∀ I,
-        OU.evaluate I =
-        (op
-          (O.evaluate (Vector.cast (by simp) (I.take n)))
-          (U.evaluate (Vector.cast (by simp) (I.take n'))))
-    } :=
-  let ⟨⟨state, root⟩, inv, ps⟩ := apply_helper op O U initial inv_initial
-  ⟨ state.size,
-    ⟨⟨cook_heap state.heap inv.1,
-    root.cook (inv.2 _ root ps.1).2.2.2.1⟩,
-    (inv.2 _ root ps.1).2.2.2.2.1⟩,
-    (inv.2 _ root ps.1).2.2.2.2.2
+set_option maxHeartbeats 300000 in
+lemma apply_helper_correct {n m n' m'} (op : (Bool → Bool → Bool)) (O : OBdd n m) (U : OBdd n' m')
+    (s0 : State n n' m m') (inv : Invariant op O.bdd.heap U.bdd.heap s0)
+    {r} (heq : r = apply_helper op O U s0) :
+    (Invariant op O.bdd.heap U.bdd.heap r.1) ∧
+    (r.1.cache[(⟨O.1.root, U.1.root⟩ : Pointer m × Pointer m')]? = some r.2) ∧
+    (s0.size ≤ r.1.size) ∧
+    (∀ (k : Pointer m × Pointer m'),
+      (∀ p, s0.cache[k]? = some p → r.1.cache[k]? = some p) ∧
+      (r.1.cache[k]? = none → s0.cache[k]? = none) ∧
+      (s0.cache[k]? = none → (∃ p, r.1.cache[k]? = some p) →
+      Pointer.Reachable O.1.heap O.1.root k.1 ∧ Pointer.Reachable U.1.heap U.1.root k.2)) := by
+  rcases heq with ⟨rfl, rfl⟩
+  fun_induction apply_helper with
+  | case1 O U s0 root hc => exact ⟨inv, hc, .refl, by grind only⟩
+  | case2 O U s0 hc b O_root_def b' U_root_def =>
+    split_ands
+    · exact insert_terminal_invariant s0 inv O_root_def U_root_def
+    · simp only [O_root_def, U_root_def, Std.HashMap.getElem?_insert_self]
+    · exact .refl
+    · intro k
+      constructor
+      · intro p hp
+        simp only [cache_get] at hc
+        rw [← hp]
+        simp only [Std.HashMap.getElem?_insert, beq_iff_eq, ite_eq_right_iff]
+        intro contra
+        subst contra
+        rw [hc] at hp
+        contradiction
+      · constructor
+        · simp only [getElem?_eq_none_iff, Std.HashMap.mem_insert, beq_iff_eq, not_or,
+            and_imp, imp_self, implies_true]
+        · rintro h1 ⟨p, hp⟩
+          simp only [Std.HashMap.getElem?_insert,beq_iff_eq] at hp
+          split at hp
+          next heq =>
+            subst heq
+            simp only [O_root_def, Pointer.Reachable.refl, U_root_def, and_self]
+          next heq => rw [h1] at hp; contradiction
+  | case3 O U s0 hc b O_root_def j' U_root_def sl rl heql sh rh heqh ihl ihh =>
+    simp only [OBdd.low_heap_eq_heap, OBdd.low_root_eq_low, OBdd.high_heap_eq_heap,
+      OBdd.high_root_eq_high, heql, heqh] at ihl ihh
+    have ⟨invl, hl, hsl, hlp⟩ := ihl inv
+    have ⟨invh, hh, hsh, hhp⟩ := ihh invl
+    let N : RawNode (max n n') := ⟨⟨U.1.heap[j'].var.1, by omega⟩, rl, rh⟩
+    let r := heap_push O U N
+    have ⟨invv, hv, hsv, hvp⟩ := heap_push_correct N rfl invh
+      (by
+        use ⟨O.1.root, U.bdd.heap[j'].low⟩
+        simp only [N]
+        exact (hhp _).1 _ hl
+      )
+      ⟨_, hh⟩
+      (by
+        simp only [N]
+        rw [O_root_def, U_root_def]
+        simp only [Fin.getElem_fin, toVar_or, le_sup_iff, Fin.is_le', or_true,
+          inf_of_le_right]
+      )
+      (by
+        simp only [N]
+        intro j hj1 hj2
+        have := (hhp _).1 _ hl
+        rw [hj2] at this
+        have that := (invh.2 _ (.inr j) this).1 _ hj1 rfl
+        simp only at that
+        rw [that]
+        exact aux_lt1_low O_root_def U_root_def
+      )
+      (by
+        intro j hj1 hj2
+        simp only [N]
+        have := (invh.2 _ _ hh).1 _ hj1 hj2
+        rw [this]
+        exact aux_lt1_high O_root_def U_root_def
+      )
+      (by
+        intro h0 h1 I
+        symm
+        simp only [OBdd.evaluate_node U_root_def, OBdd.evaluate_terminal O_root_def]
+        rw [op_if1 op]
+        simp only [Nat.sub_zero, Fin.getElem_fin, Vector.getElem_cast, cook_heap,
+          RawNode.cook, Pointer.node.injEq, OBdd.evaluate_node, Vector.getElem_ofFn,
+          Vector.getElem_push_eq]
+        congr 1
+        · grind only [= Fin.getElem_fin, Vector.getElem_extract]
+        · conv =>
+            rhs
+            congr
+            congr
+            congr
+            rfl
+            simp [cook_heap, RawNode.cook]
+            rfl
+          symm
+          have h := invh.2 ⟨O.1.root, U.bdd.heap[j'].high⟩ rh hh
+          rcases h with ⟨h1, h2, h3, h4, h5, h6⟩
+          simp only [OBdd.mk_eq_self, Vector.take_eq_extract, OBdd.mk_eq_high U_root_def] at h6
+          rw [O.evaluate_terminal O_root_def] at h6
+          rw [push_evaluate (by rw [OBdd.high_heap_eq_heap]; rfl) (h0 := h0) (ho := h5)]
+          · exact h6 I
+          · simp only [OBdd.high_root_eq_high, Fin.getElem_fin, Vector.getElem_ofFn,
+              Vector.getElem_push_eq, N]
+          · grind only [RawPointer.Bounded]
+        · conv =>
+            rhs
+            congr
+            congr
+            congr
+            rfl
+            simp [cook_heap, RawNode.cook]
+            rfl
+          symm
+          have : sh.cache[(⟨O.1.root, U.bdd.heap[j'].low⟩ : Pointer m × Pointer m')]? = some rl := by
+            apply (hhp _).1
+            exact hl
+          have h := invh.2 ⟨O.1.root, U.bdd.heap[j'].low⟩ rl this
+          rcases h with ⟨h1, h2, h3, h4, h5, h6⟩
+          simp only [OBdd.mk_eq_self, Vector.take_eq_extract, U.mk_eq_low U_root_def] at h6
+          rw [O.evaluate_terminal O_root_def] at h6
+          rw [push_evaluate (by rw [OBdd.low_heap_eq_heap]; rfl) (h0 := h0) (ho := h5)]
+          · exact h6 I
+          · simp only [OBdd.low_root_eq_low, Fin.getElem_fin, Vector.getElem_ofFn,
+              Vector.getElem_push_eq, N]
+          · grind only [RawPointer.Bounded]
+      )
+      (by
+        simp only [cache_get] at hc
+        cases heq : sh.cache[(⟨O.1.root, U.1.root⟩ : Pointer m × Pointer m')]? with
+        | none => rfl
+        | some val =>
+          cases heqq : sl.cache[(⟨O.1.root, U.1.root⟩ : Pointer m × Pointer m')]? with
+          | none =>
+            absurd ((hhp _).2.2 heqq ⟨val, heq⟩).2
+            exact OBdd.not_reachable_high_root U_root_def
+          | some val =>
+            absurd ((hlp _).2.2 hc ⟨_, heqq⟩).2
+            exact OBdd.not_reachable_low_root U_root_def
+      )
+    split_ands
+    · exact invv
+    · exact hv
+    · exact .trans hsl (.trans hsh hsv)
+    · intro k
+      constructor
+      · intro p hp
+        apply (hvp _).1
+        apply (hhp _).1
+        apply (hlp _).1
+        exact hp
+      · constructor
+        · intro hk
+          apply (hlp _).2.1
+          apply (hhp _).2.1
+          apply (hvp _).2.1
+          exact hk
+        · intro hk hkp
+          cases heq : sh.cache[k]? with
+          | none =>
+            apply (hvp _).2.2 heq hkp
+          | some w =>
+            cases heqq : sl.cache[k]? with
+            | none =>
+              have := (hhp _).2.2 heqq ⟨_, heq⟩
+              constructor
+              · exact this.1
+              · exact .trans (U.bdd.reachable_high U_root_def) this.2
+            | some ww =>
+              have := (hlp _).2.2 hk ⟨_, heqq⟩
+              constructor
+              · exact this.1
+              · exact .trans (U.bdd.reachable_low U_root_def) this.2
+  | case4 O U s0 hc j O_root_def b' U_root_def sl rl heql sh rh heqh ihl ihh=>
+    simp only [OBdd.low_heap_eq_heap, OBdd.low_root_eq_low, OBdd.high_heap_eq_heap,
+      OBdd.high_root_eq_high, heql, heqh] at ihl ihh
+    have ⟨invl, hl, hsl, hlp⟩ := ihl inv
+    have ⟨invh, hh, hsh, hhp⟩ := ihh invl
+    let N : RawNode (max n n') := ⟨⟨O.1.heap[j].var.1, by omega⟩, rl, rh⟩
+    let r := heap_push O U N
+    have ⟨invv, hv, hsv, hvp⟩ := heap_push_correct N rfl invh
+      ⟨_, (hhp _).1 _ hl⟩
+      ⟨_, hh⟩
+      (by
+        simp only [N]
+        rw [O_root_def, U_root_def]
+        simp only [Fin.getElem_fin, toVar_or, le_sup_iff, Fin.is_le', true_or, inf_of_le_left]
+      )
+      (by
+        simp only [N]
+        intro j hj1 hj2
+        have := (hhp _).1 _ hl
+        rw [hj2] at this
+        have that := (invh.2 _ (.inr j) this).1 _ hj1 rfl
+        simp only at that
+        rw [that]
+        exact aux_lt2_low O_root_def U_root_def
+      )
+      (by
+        simp only [N]
+        intro j hj1 hj2
+        have := (invh.2 _ _ hh).1 _ hj1 hj2
+        rw [this]
+        exact aux_lt2_high O_root_def U_root_def
+      )
+      (by
+        intro h0 h1 I
+        symm
+        simp only [OBdd.evaluate_node O_root_def, OBdd.evaluate_terminal U_root_def]
+        rw [op_if2 op]
+        simp only [Nat.sub_zero, Fin.getElem_fin, Vector.getElem_cast, cook_heap,
+          RawNode.cook, Pointer.node.injEq, OBdd.evaluate_node, Vector.getElem_ofFn,
+          Vector.getElem_push_eq]
+        congr 1
+        · grind only [= Fin.getElem_fin, Vector.getElem_extract]
+        · conv =>
+            rhs
+            congr
+            congr
+            congr
+            rfl
+            simp [cook_heap, RawNode.cook]
+            rfl
+          symm
+          have h := invh.2 ⟨O.bdd.heap[j].high, U.1.root⟩ rh hh
+          rcases h with ⟨h1, h2, h3, h4, h5, h6⟩
+          simp only [O.mk_eq_high O_root_def, Vector.take_eq_extract, OBdd.mk_eq_self,
+            U.evaluate_terminal U_root_def] at h6
+          rw [push_evaluate (by rw [OBdd.high_heap_eq_heap]; rfl) (h0 := h0) (ho := h5)]
+          · exact h6 I
+          · simp only [Fin.getElem_fin, OBdd.high_root_eq_high, Vector.getElem_ofFn,
+              Vector.getElem_push_eq, N]
+          · grind only [RawPointer.Bounded]
+        · conv =>
+            rhs
+            congr
+            congr
+            congr
+            rfl
+            simp [cook_heap, RawNode.cook]
+            rfl
+          symm
+          have : sh.cache[(⟨O.bdd.heap[j].low, U.1.root⟩ : Pointer m × Pointer m')]? = some rl := by
+            apply (hhp _).1
+            exact hl
+          have h := invh.2 ⟨O.bdd.heap[j].low, U.1.root⟩ rl this
+          rcases h with ⟨h1, h2, h3, h4, h5, h6⟩
+          simp only [OBdd.mk_eq_low O_root_def, Vector.take_eq_extract, OBdd.mk_eq_self,
+            U.evaluate_terminal U_root_def] at h6
+          rw [push_evaluate (by rw [OBdd.low_heap_eq_heap]; rfl) (h0 := h0) (ho := h5)]
+          · exact h6 I
+          · simp only [OBdd.low_root_eq_low, Fin.getElem_fin, Vector.getElem_ofFn,
+              Vector.getElem_push_eq, N]
+          · grind only [RawPointer.Bounded]
+      )
+      (by
+        simp only [cache_get] at hc
+        cases heq : sh.cache[(⟨O.1.root, U.1.root⟩ : Pointer m × Pointer m')]? with
+        | none => rfl
+        | some val =>
+          cases heqq : sl.cache[(⟨O.1.root, U.1.root⟩ : Pointer m × Pointer m')]? with
+          | none =>
+            absurd ((hhp _).2.2 heqq ⟨val, heq⟩).1
+            exact OBdd.not_reachable_high_root O_root_def
+          | some val =>
+            absurd ((hlp _).2.2 hc ⟨_, heqq⟩).1
+            exact OBdd.not_reachable_low_root O_root_def
+      )
+    split_ands
+    · exact invv
+    · exact hv
+    · exact .trans hsl (.trans hsh hsv)
+    · intro k
+      constructor
+      · intro p hp
+        apply (hvp _).1
+        apply (hhp _).1
+        apply (hlp _).1
+        exact hp
+      · constructor
+        · intro hk
+          apply (hlp _).2.1
+          apply (hhp _).2.1
+          apply (hvp _).2.1
+          exact hk
+        · intro hk hkp
+          cases heq : sh.cache[k]? with
+          | none =>
+            apply (hvp _).2.2 heq hkp
+          | some w =>
+            cases heqq : sl.cache[k]? with
+            | none =>
+              have := (hhp _).2.2 heqq ⟨_, heq⟩
+              constructor
+              · exact .trans (O.bdd.reachable_high O_root_def) this.1
+              · exact this.2
+            | some ww =>
+              have := (hlp _).2.2 hk ⟨_, heqq⟩
+              constructor
+              · exact .trans (O.bdd.reachable_low O_root_def) this.1
+              · exact this.2
+  | case5 O U s0 hc j O_root_def j' U_root_def hlt sl rl heql sh rh heqh ihl ihh =>
+    simp only [OBdd.low_heap_eq_heap, OBdd.low_root_eq_low, OBdd.high_heap_eq_heap,
+      OBdd.high_root_eq_high, heql, heqh] at ihl ihh
+    have ⟨invl, hl, hsl, hlp⟩ := ihl inv
+    have ⟨invh, hh, hsh, hhp⟩ := ihh invl
+    let N : RawNode (max n n') := ⟨⟨O.1.heap[j].var.1, by omega⟩, rl, rh⟩
+    let r := heap_push O U N
+    have ⟨invv, hv, hsv, hvp⟩ := heap_push_correct N rfl invh
+      ⟨_, (hhp _).1 _ hl⟩
+      ⟨_, hh⟩
+      (by
+        simp only [N]
+        rw [O_root_def, U_root_def]
+        simp only [Fin.getElem_fin, toVar_or]
+        exact Eq.symm (min_eq_left_of_lt hlt)
+      )
+      (by
+        simp only [N]
+        intro j'' hj1 hj2
+        have := (hhp _).1 _ hl
+        rw [hj2] at this
+        have that := (invh.2 _ _ this).1 _ hj1 rfl
+        simp only at that
+        rw [that]
+        exact aux_lt3_low O_root_def U_root_def hlt
+      )
+      (by
+        simp only [N]
+        intro j'' hj1 hj2
+        have := (invh.2 _ _ hh).1 _ hj1 hj2
+        rw [this]
+        exact aux_lt3_high O_root_def U_root_def hlt
+      )
+      (by
+        intro h0 h1 I
+        symm
+        simp only [OBdd.evaluate_node O_root_def, OBdd.evaluate_node U_root_def]
+        rw [op_if2 op]
+        simp only [Nat.sub_zero, Fin.getElem_fin, Vector.getElem_cast, cook_heap,
+          RawNode.cook, Pointer.node.injEq, OBdd.evaluate_node, Vector.getElem_ofFn,
+          Vector.getElem_push_eq]
+        congr 1
+        · grind only [usr Fin.isLt, = Fin.getElem_fin, Vector.getElem_extract]
+        · conv =>
+            rhs
+            congr
+            congr
+            congr
+            rfl
+            simp [cook_heap, RawNode.cook]
+            rfl
+          symm
+          have h := invh.2 ⟨O.bdd.heap[j].high, U.1.root⟩ rh hh
+          rcases h with ⟨h1, h2, h3, h4, h5, h6⟩
+          simp only [OBdd.mk_eq_high O_root_def, Vector.take_eq_extract, OBdd.mk_eq_self] at h6
+          rw [push_evaluate (by rw [OBdd.high_heap_eq_heap]; rfl) (h0 := h0) (ho := h5)]
+          · simp_all only [Fin.getElem_fin, Pointer.node.injEq, OBdd.evaluate_node,
+              Vector.getElem_cast]
+          · simp only [OBdd.high_root_eq_high, Fin.getElem_fin, Vector.getElem_ofFn,
+              Vector.getElem_push_eq, N]
+          · grind only [RawPointer.Bounded]
+        · conv =>
+            rhs
+            congr
+            congr
+            congr
+            rfl
+            simp [cook_heap, RawNode.cook]
+            rfl
+          symm
+          have : sh.cache[(⟨O.bdd.heap[j].low, U.1.root⟩ : Pointer m × Pointer m')]? = some rl := by
+            apply (hhp _).1
+            exact hl
+          have h := invh.2 ⟨O.bdd.heap[j].low, U.1.root⟩ rl this
+          rcases h with ⟨h1, h2, h3, h4, h5, h6⟩
+          simp only [O.mk_eq_low O_root_def, Vector.take_eq_extract, OBdd.mk_eq_self] at h6
+          rw [push_evaluate (by rw [OBdd.low_heap_eq_heap]; rfl) (h0 := h0) (ho := h5)]
+          · simp_all only [Fin.getElem_fin, Pointer.node.injEq, OBdd.evaluate_node,
+              Vector.getElem_cast]
+          · simp only [OBdd.low_root_eq_low, Fin.getElem_fin, Vector.getElem_ofFn,
+              Vector.getElem_push_eq, N]
+          · grind only [RawPointer.Bounded]
+      )
+      (by
+        simp only [cache_get] at hc
+        cases heq : sh.cache[(⟨O.1.root, U.1.root⟩ : Pointer m × Pointer m')]? with
+        | none => rfl
+        | some val =>
+          cases heqq : sl.cache[(⟨O.1.root, U.1.root⟩ : Pointer m × Pointer m')]? with
+          | none =>
+            absurd ((hhp _).2.2 heqq ⟨val, heq⟩).1
+            exact OBdd.not_reachable_high_root O_root_def
+          | some val =>
+            absurd ((hlp _).2.2 hc ⟨_, heqq⟩).1
+            exact OBdd.not_reachable_low_root O_root_def
+      )
+    split_ands
+    · exact invv
+    · exact hv
+    · exact .trans hsl (.trans hsh hsv)
+    · intro k
+      constructor
+      · intro p hp
+        apply (hvp _).1
+        apply (hhp _).1
+        apply (hlp _).1
+        exact hp
+      · constructor
+        · intro hk
+          apply (hlp _).2.1
+          apply (hhp _).2.1
+          apply (hvp _).2.1
+          exact hk
+        · intro hk hkp
+          cases heq : sh.cache[k]? with
+          | none =>
+            apply (hvp _).2.2 heq hkp
+          | some w =>
+            cases heqq : sl.cache[k]? with
+            | none =>
+              have := (hhp _).2.2 heqq ⟨_, heq⟩
+              constructor
+              · exact .trans (O.bdd.reachable_high O_root_def) this.1
+              · exact this.2
+            | some ww =>
+              have := (hlp _).2.2 hk ⟨_, heqq⟩
+              constructor
+              · exact .trans (O.bdd.reachable_low O_root_def) this.1
+              · exact this.2
+  | case6 O U s0 hc j O_root_def j' U_root_def _ hgt sl rl heql sh rh heqh ihl ihh =>
+    simp only [OBdd.low_heap_eq_heap, OBdd.low_root_eq_low, OBdd.high_heap_eq_heap,
+      OBdd.high_root_eq_high, heql, heqh] at ihl ihh
+    have ⟨invl, hl, hsl, hlp⟩ := ihl inv
+    have ⟨invh, hh, hsh, hhp⟩ := ihh invl
+    let N : RawNode (max n n') := ⟨⟨U.1.heap[j'].var.1, by omega⟩, rl, rh⟩
+    let r := heap_push O U N
+    have ⟨invv, hv, hsv, hvp⟩ := heap_push_correct N rfl invh
+      ⟨_, (hhp _).1 _ hl⟩
+      ⟨_, hh⟩
+      (by
+        simp only [N]
+        rw [O_root_def, U_root_def]
+        simp only [Fin.getElem_fin, toVar_or]
+        exact Eq.symm (min_eq_right_of_lt hgt)
+      )
+      (by
+        simp only [N]
+        intro j'' hj1 hj2
+        have := (hhp _).1 _ hl
+        rw [hj2] at this
+        have that := (invh.2 _ _ this).1 _ hj1 rfl
+        simp only at that
+        rw [that]
+        exact aux_lt4_low O_root_def U_root_def hgt
+      )
+      (by
+        simp only [N]
+        intro j'' hj1 hj2
+        have := (invh.2 _ _ hh).1 _ hj1 hj2
+        rw [this]
+        exact aux_lt4_high O_root_def U_root_def hgt
+      )
+      (by
+        intro h0 h1 I
+        symm
+        simp only [OBdd.evaluate_node O_root_def, OBdd.evaluate_node U_root_def]
+        rw [op_if1 op]
+        simp only [Nat.sub_zero, Fin.getElem_fin, Vector.getElem_cast, cook_heap,
+          RawNode.cook, Pointer.node.injEq, OBdd.evaluate_node, Vector.getElem_ofFn,
+          Vector.getElem_push_eq]
+        congr 1
+        · grind only [usr Fin.isLt, = Fin.getElem_fin, Vector.getElem_extract]
+        · conv =>
+            rhs
+            congr
+            congr
+            congr
+            rfl
+            simp [cook_heap, RawNode.cook]
+            rfl
+          symm
+          have h := invh.2 ⟨O.1.root, U.bdd.heap[j'].high⟩ rh hh
+          rcases h with ⟨h1, h2, h3, h4, h5, h6⟩
+          simp only [OBdd.mk_eq_self, Vector.take_eq_extract, U.mk_eq_high U_root_def] at h6
+          rw [push_evaluate (by rw [OBdd.high_heap_eq_heap]; rfl) (h0 := h0) (ho := h5)]
+          · simp_all only [Fin.getElem_fin, Pointer.node.injEq, OBdd.evaluate_node,
+              Vector.getElem_cast]
+          · simp only [OBdd.high_root_eq_high, Fin.getElem_fin, Vector.getElem_ofFn,
+              Vector.getElem_push_eq, N]
+          · grind only [RawPointer.Bounded]
+        · conv =>
+            rhs
+            congr
+            congr
+            congr
+            rfl
+            simp [cook_heap, RawNode.cook]
+            rfl
+          symm
+          have : sh.cache[(⟨O.1.root, U.bdd.heap[j'].low⟩ : Pointer m × Pointer m')]? = some rl := by
+            apply (hhp _).1
+            exact hl
+          have h := invh.2 ⟨O.1.root, U.bdd.heap[j'].low⟩ rl this
+          rcases h with ⟨h1, h2, h3, h4, h5, h6⟩
+          simp only [OBdd.mk_eq_self, Vector.take_eq_extract, U.mk_eq_low U_root_def] at h6
+          rw [push_evaluate (by rw [OBdd.low_heap_eq_heap]; rfl) (h0 := h0) (ho := h5)]
+          · simp_all only [Fin.getElem_fin, Pointer.node.injEq, OBdd.evaluate_node,
+              Vector.getElem_cast]
+          · simp only [OBdd.low_root_eq_low, Fin.getElem_fin, Vector.getElem_ofFn,
+              Vector.getElem_push_eq, N]
+          · grind only [RawPointer.Bounded]
+      )
+      (by
+        simp only [cache_get] at hc
+        cases heq : sh.cache[(⟨O.1.root, U.1.root⟩ : Pointer m × Pointer m')]? with
+        | none => rfl
+        | some val =>
+          cases heqq : sl.cache[(⟨O.1.root, U.1.root⟩ : Pointer m × Pointer m')]? with
+          | none =>
+            absurd ((hhp _).2.2 heqq ⟨val, heq⟩).2
+            exact OBdd.not_reachable_high_root U_root_def
+          | some val =>
+            absurd ((hlp _).2.2 hc ⟨_, heqq⟩).2
+            exact OBdd.not_reachable_low_root U_root_def
+      )
+    split_ands
+    · exact invv
+    · exact hv
+    · exact .trans hsl (.trans hsh hsv)
+    · intro k
+      constructor
+      · intro p hp
+        apply (hvp _).1
+        apply (hhp _).1
+        apply (hlp _).1
+        exact hp
+      · constructor
+        · intro hk
+          apply (hlp _).2.1
+          apply (hhp _).2.1
+          apply (hvp _).2.1
+          exact hk
+        · intro hk hkp
+          cases heq : sh.cache[k]? with
+          | none =>
+            apply (hvp _).2.2 heq hkp
+          | some w =>
+            cases heqq : sl.cache[k]? with
+            | none =>
+              have := (hhp _).2.2 heqq ⟨_, heq⟩
+              constructor
+              · exact this.1
+              · exact .trans (U.bdd.reachable_high U_root_def) this.2
+            | some ww =>
+              have := (hlp _).2.2 hk ⟨_, heqq⟩
+              constructor
+              · exact this.1
+              · exact .trans (U.bdd.reachable_low U_root_def) this.2
+
+  | case7 O U s0 hc j O_root_def j' U_root_def _ hgt sl rl heql sh rh heqh ihl ihh =>
+    simp only [OBdd.low_heap_eq_heap, OBdd.low_root_eq_low, OBdd.high_heap_eq_heap,
+      OBdd.high_root_eq_high, heql, heqh] at ihl ihh
+    have ⟨invl, hl, hsl, hlp⟩ := ihl inv
+    have ⟨invh, hh, hsh, hhp⟩ := ihh invl
+    let N : RawNode (max n n') := ⟨⟨U.1.heap[j'].var.1, by omega⟩, rl, rh⟩
+    let r := heap_push O U N
+    have ⟨invv, hv, hsv, hvp⟩ := heap_push_correct N rfl invh
+      ⟨_, (hhp _).1 _ hl⟩
+      ⟨_, hh⟩
+      (by
+        simp only [N]
+        rw [O_root_def, U_root_def]
+        simp only [Fin.getElem_fin, toVar_or]
+        have heeq : O.1.heap[j].var.1 = U.1.heap[j'].var.1 := by omega
+        simp only [Fin.getElem_fin] at heeq
+        rw [heeq]
+        simp only [min_self]
+      )
+      (by
+        simp only [N]
+        intro j'' hj1 hj2
+        have := (hhp _).1 _ hl
+        rw [hj2] at this
+        have that := (invh.2 _ _ this).1 _ hj1 rfl
+        simp only at that
+        rw [that]
+        exact aux_lt5_low O_root_def U_root_def (by omega)
+      )
+      (by
+        simp only [N]
+        intro j'' hj1 hj2
+        have := (invh.2 _ _ hh).1 _ hj1 hj2
+        rw [this]
+        exact aux_lt5_high O_root_def U_root_def (by omega)
+      )
+      (by
+        intro h0 h1 I
+        symm
+        simp only [OBdd.evaluate_node U_root_def, OBdd.evaluate_node O_root_def]
+        have heeq : O.1.heap[j].var.1 = U.1.heap[j'].var.1 := by omega
+        have heo := Vector.getElem_extract (as := I) (start := 0) (stop := n) (i := O.1.heap[j.1].var.1) (by omega)
+        have heu := Vector.getElem_extract (as := I) (start := 0) (stop := n') (i := U.1.heap[j'.1].var.1) (by omega)
+        have : (Vector.cast (m := n') (by omega) (I.extract 0 n'))[U.1.heap[j'].var] = (Vector.cast (m := n) (by omega) (I.extract 0 n))[O.1.heap[j].var] := by
+          simp only [Fin.getElem_fin]
+          rw [Vector.getElem_cast]
+          rw [Vector.getElem_cast]
+          rw [heo]
+          rw [heu]
+          simp only [zero_add]
+          congr 1
+          symm
+          exact heeq
+        rw [this]
+        rw [op_if3 op]
+        simp only [Nat.sub_zero, Fin.getElem_fin, Vector.getElem_cast, cook_heap,
+          RawNode.cook, Pointer.node.injEq, OBdd.evaluate_node, Vector.getElem_ofFn,
+          Vector.getElem_push_eq]
+        congr 1
+        · grind only [usr Fin.isLt, = Fin.getElem_fin]
+        · conv =>
+            rhs
+            congr
+            congr
+            congr
+            rfl
+            simp [cook_heap, RawNode.cook]
+            rfl
+          symm
+          have h := invh.2 ⟨O.bdd.heap[j].high, U.bdd.heap[j'].high⟩ rh hh
+          rcases h with ⟨h1, h2, h3, h4, h5, h6⟩
+          simp only [OBdd.mk_eq_high O_root_def, OBdd.mk_eq_high U_root_def] at h6
+          rw [push_evaluate (by rw [OBdd.high_heap_eq_heap]; rfl) (h0 := h0) (ho := h5)]
+          · exact h6 I
+          · simp only [OBdd.high_root_eq_high, Fin.getElem_fin, Vector.getElem_ofFn,
+              Vector.getElem_push_eq, N]
+          · grind only [RawPointer.Bounded]
+        · conv =>
+            rhs
+            congr
+            congr
+            congr
+            rfl
+            simp [cook_heap, RawNode.cook]
+            rfl
+          symm
+          have : sh.cache[(⟨O.bdd.heap[j].low, U.bdd.heap[j'].low⟩ : Pointer m × Pointer m')]? = some rl := by
+            apply (hhp _).1
+            exact hl
+          have h := invh.2 ⟨O.bdd.heap[j].low, U.bdd.heap[j'].low⟩ rl this
+          rcases h with ⟨h1, h2, h3, h4, h5, h6⟩
+          simp only [OBdd.mk_eq_low O_root_def, OBdd.mk_eq_low U_root_def] at h6
+          rw [push_evaluate (by rw [OBdd.low_heap_eq_heap]; rfl) (h0 := h0) (ho := h5)]
+          · exact h6 I
+          · simp only [Fin.getElem_fin, OBdd.low_root_eq_low, Vector.getElem_ofFn,
+              Vector.getElem_push_eq, N]
+          · grind only [RawPointer.Bounded]
+      )
+      (by
+        simp only [cache_get] at hc
+        cases heq : sh.cache[(⟨O.1.root, U.1.root⟩ : Pointer m × Pointer m')]? with
+        | none => rfl
+        | some val =>
+          cases heqq : sl.cache[(⟨O.1.root, U.1.root⟩ : Pointer m × Pointer m')]? with
+          | none =>
+            absurd ((hhp _).2.2 heqq ⟨val, heq⟩).2
+            exact OBdd.not_reachable_high_root U_root_def
+          | some val =>
+            absurd ((hlp _).2.2 hc ⟨_, heqq⟩).2
+            exact OBdd.not_reachable_low_root U_root_def
+      )
+    split_ands
+    · exact invv
+    · exact hv
+    · exact .trans hsl (.trans hsh hsv)
+    · intro k
+      constructor
+      · intro p hp
+        apply (hvp _).1
+        apply (hhp _).1
+        apply (hlp _).1
+        exact hp
+      · constructor
+        · intro hk
+          apply (hlp _).2.1
+          apply (hhp _).2.1
+          apply (hvp _).2.1
+          exact hk
+        · intro hk hkp
+          cases heq : sh.cache[k]? with
+          | none =>
+            apply (hvp _).2.2 heq hkp
+          | some w =>
+            cases heqq : sl.cache[k]? with
+            | none =>
+              have := (hhp _).2.2 heqq ⟨_, heq⟩
+              constructor
+              · exact .trans (O.bdd.reachable_high O_root_def) this.1
+              · exact .trans (U.bdd.reachable_high U_root_def) this.2
+            | some ww =>
+              have := (hlp _).2.2 hk ⟨_, heqq⟩
+              constructor
+              · exact .trans (O.bdd.reachable_low O_root_def) this.1
+              · exact .trans (U.bdd.reachable_low U_root_def) this.2
+
+public def oapply {n m n' m'} (op : Bool → Bool → Bool) (O : OBdd n m) (U : OBdd n' m') :
+    (s : Nat) × OBdd (n ⊔ n') s :=
+  let r := apply_helper op O U initial
+  have ⟨inv, ps⟩ := apply_helper_correct op O U initial inv_initial rfl
+  ⟨ r.1.size,
+    ⟨⟨cook_heap r.1.heap inv.1,
+    r.2.cook (inv.2 _ r.2 ps.1).2.2.2.1⟩,
+    (inv.2 _ r.2 ps.1).2.2.2.2.1⟩,
   ⟩
+
+public lemma oapply_correct {n m n' m'} (op : Bool → Bool → Bool) (O : OBdd n m) (U : OBdd n' m') :
+    ∀ I, (oapply op O U).2.evaluate I = op
+      (O.evaluate (Vector.cast (by simp) (I.take n)))
+      (U.evaluate (Vector.cast (by simp) (I.take n'))) := by
+  let r := apply_helper op O U initial
+  have ⟨h1, h2, h3⟩ := apply_helper_correct op O U initial inv_initial rfl
+  rw [oapply]
+  split
+  exact (h1.2 _ r.2 h2).2.2.2.2.2
 
 end Apply
